Working on trace_preservation

Multimap.v
@@ -1,3 +1,4 @@
+From Coq Require Import Lists.List.
 
 Local Definition map' (K V : Type) :=
   prod (K -> V) (K -> K -> bool).
@@ -7,20 +8,25 @@ Local Definition empty' {K V : Type} v eqb : map' K V := (fun _ => v, eqb).
 Local Definition update' {K V : Type} (m : map' K V) k v :=
   (fun k' => if (snd m) k k' then v else (fst m) k', snd m).
 
+Local Definition map (K V : Type) := map' K (option V).
 
-Definition map (K V : Type) := map' K (option V).
+Local Definition empty {K V : Type} eqb : map K V := empty' None eqb.
 
-Definition empty {K V : Type} eqb : map K V := empty' None eqb.
-
-Definition update {K V : Type} (m : map K V) k v :=
+Local Definition update {K V : Type} (m : map K V) k v :=
   update' m k (Some v).
 
-Definition lookup {K V : Type} (m : map K V) k := (fst m) k.
+Local Definition lookup {K V : Type} (m : map K V) k := (fst m) k.
 
+Definition multimap (K V : Type) := map' K (list V).
 
-Definition multimap (K V : Type) := map K (map' V V).
+Definition multimap_empty {K V : Type} eqb : multimap K V :=
+  empty' nil eqb.
 
-(*
-Definition multimap_empty {K V : Type} eqbk eqbv :=
-  empty' (empty  V) nil eqb.
-*)
+Definition multimap_lookup {K V : Type} (m : multimap K V) k : list V :=
+  fst m k.
+
+Definition multimap_contains {K V : Type} (m : multimap K V) k v : Prop :=
+  In v (multimap_lookup m k).
+
+Definition multimap_update {K V : Type} (m : multimap K V) k v :=
+  update' m k (v :: multimap_lookup m k).
